Exemplar/Monad.lean
@@ -1,0 +1,64 @@
+import Mathlib.Data.List.Basic
+import Std.Data.Iterators.Producers
+import Std.Data.Iterators.Combinators.Zip
+
+def mktwo (a:Nat) (b:Nat) : List Nat := [a, b ]
+
+def double (a:Nat) : Nat := a + a
+
+def first := [1, 2, 3]
+def second := [4, 5, 6]
+
+#eval (· , ·) 1 2
+
+#eval [mktwo] <*> first <*> first
+#eval [([· , ·])] <*> first <*> second
+
+#check [mktwo]
+
+#eval [double] <*> first  -- [2, 4, 6]
+
+def fpo := do
+  pure (1 + (<-first))
+
+def fprod {α} [Mul α] (x : List α) (y : List α) : List α := do
+      pure ((<-x) * (<-y))
+
+def prod {α} [Mul α] (x : List α) (y : List α) : List (List α) := do
+  let ax <- x
+  pure do
+    let ay <- y
+    pure (ax * ay)
+
+#eval fprod first second
+
+#eval prod first second
+
+class Zippable (coll: Type -> Type) where
+  zip : coll α → coll β → coll (α × β)
+
+def inner [HMul α β γ] [Monad M] [Zippable M] (x : M α) (y : M β) : M γ := do
+  let (ax, ay) <- Zippable.zip x y
+  pure (ax * ay)
+
+instance : Zippable List where
+  zip  := List.zip
+
+#eval inner first second
+-- examples of some unsafe coercions
+
+instance [Monad M]: Coe α (M α) where
+  coe α := pure α
+
+#check ( (· + 1) : List (Nat->Nat))
+
+def x :=  1
+
+#eval ( x: List Nat)
+#eval ( x: Option Nat)
+#eval ( x: Except String Nat)
+
+instance [Monad M]: OfNat (M Nat) n where
+  ofNat := (n: M Nat)
+
+#eval ( 1: List Nat)
